simplify hist wps

src/program_proof/pav/history.v
@@ -8,22 +8,23 @@ Context `{!heapGS Σ, !pavG Σ}.
 
 (* TODO: maybe only cliG version needed. not pure or adtrG. *)
 Definition know_hist_val_cliG cli_γ (uid ep : w64) (lat : lat_val_ty) : iProp Σ :=
-  let len_vals := match lat with None => 0%nat | Some (ver, val) => S $ uint.nat ver end in
   ∃ vals,
-  "%Hlen_vals" ∷ ⌜ length vals = len_vals ⌝ ∗
   "%Hbound_vals" ∷ ⌜ length vals < 2^64 ⌝ ∗
-  "%Hlook_lat" ∷ ⌜ last vals = snd <$> lat ⌝ ∗
+  "%Hlook_lat" ∷ ⌜ last vals = lat ⌝ ∗
+  (* prior vers exist in prior or this map. *)
   "#Hhist" ∷ ([∗ list] ver ↦ '(prior, pk) ∈ vals,
     (∃ dig m_γ comm,
     "%Hlt_prior" ∷ ⌜ uint.Z prior ≤ uint.Z ep ⌝ ∗
     "#Hsubmap" ∷ mono_list_idx_own cli_γ (uint.nat prior) (Some (dig, m_γ)) ∗
     "#Hin_prior" ∷ (uid, W64 ver) ↪[m_γ]□ Some (prior, comm) ∗
     "#Hcomm" ∷ is_comm pk comm)) ∗
-  ( "Hnin_nextver" ∷ (∃ (bound : w64) dig m_γ,
+  ( (* next ver doesn't exist in this or later map. *)
+    "Hnin_nextver" ∷ (∃ (bound : w64) dig m_γ,
       "%Hgte_bound" ∷ ⌜ uint.Z ep ≤ uint.Z bound ⌝ ∗
       "#Hsubmap" ∷ mono_list_idx_own cli_γ (uint.nat bound) (Some (dig, m_γ)) ∗
       "#Hin_bound" ∷ (uid, W64 $ length vals) ↪[m_γ] None)
     ∨
+    (* next ver exists in later map. *)
     "Hin_nextver" ∷ (∃ (bound : w64) dig m_γ comm,
       "%Hgt_bound" ∷ ⌜ uint.Z ep < uint.Z bound ⌝ ∗
       "#Hsubmap" ∷ mono_list_idx_own cli_γ (uint.nat bound) (Some (dig, m_γ)) ∗
@@ -34,85 +35,67 @@ Definition know_hist_cliG cli_γ (uid : w64) (hist : list lat_val_ty) : iProp Σ
 
 End core_iprop.
 
-Module HistEntry.
-Record t :=
-  mk {
-    Epoch: w64;
-    HistVal: list w8;
-  }.
-Section defs.
+Section HistEntry.
 Context `{!heapGS Σ}.
-Definition own (ptr : loc) (obj : t) : iProp Σ :=
+Definition own_HistEntry (ptr : loc) (obj : map_val_ty) : iProp Σ :=
   ∃ sl_HistVal,
-  "Hptr_Epoch" ∷ ptr ↦[HistEntry :: "Epoch"] #obj.(Epoch) ∗
+  "Hptr_Epoch" ∷ ptr ↦[HistEntry :: "Epoch"] #obj.1 ∗
   "Hptr_HistVal" ∷ ptr ↦[HistEntry :: "HistVal"] (slice_val sl_HistVal) ∗
-  "#Hsl_HistVal" ∷ own_slice_small sl_HistVal byteT DfracDiscarded obj.(HistVal).
-End defs.
+  "#Hsl_HistVal" ∷ own_slice_small sl_HistVal byteT DfracDiscarded obj.2.
 End HistEntry.
 
 Section hist.
 Context `{!heapGS Σ, !pavG Σ}.
 
-Definition get_lat (phys : list HistEntry.t) (ep : w64) : lat_val_ty :=
-  let hist := (filter (λ x, uint.Z x.(HistEntry.Epoch) ≤ uint.Z ep) phys) in
-  (λ x, (W64 $ pred $ length hist, (x.(HistEntry.Epoch), x.(HistEntry.HistVal)))) <$> (last hist).
+Definition get_lat (phys : list map_val_ty) (ep : w64) : lat_val_ty :=
+  last $ filter (λ x, uint.Z x.1 ≤ uint.Z ep) phys.
 
-Definition phys_logic_reln (phys : list HistEntry.t) (logic : list lat_val_ty) :=
-  (∀ (ep : w64) lat, logic !! uint.nat ep = Some lat → lat = get_lat phys ep) ∧
-  length logic = match last phys with None => 0%nat | Some x => S $ uint.nat x.(HistEntry.Epoch) end.
+Definition phys_logic_reln phys (logic : list lat_val_ty) :=
+  (∀ (ep : w64) lat, logic !! uint.nat ep = Some lat → lat = get_lat phys ep).
 
-Definition own_hist cli_γ uid sl_hist (hist : list HistEntry.t) : iProp Σ :=
+Definition own_hist cli_γ uid sl_hist phys_hist : iProp Σ :=
   ∃ dim0_hist logic_hist,
   "Hsl_hist" ∷ own_slice sl_hist ptrT (DfracOwn 1) dim0_hist ∗
-  "Hdim0_hist" ∷ ([∗ list] p;o ∈ dim0_hist;hist, HistEntry.own p o) ∗
-  "%Hlogic_reln" ∷ ⌜ phys_logic_reln hist logic_hist ⌝ ∗
+  "Hdim0_hist" ∷ ([∗ list] p;o ∈ dim0_hist;phys_hist, own_HistEntry p o) ∗
+  "%Hlogic_reln" ∷ ⌜ phys_logic_reln phys_hist logic_hist ⌝ ∗
   "#Hknow_hist" ∷ know_hist_cliG cli_γ uid logic_hist.
 End hist.
 
 Section wps.
 Context `{!heapGS Σ, !pavG Σ}.
 
-Lemma wp_put_hist cli_γ uid sl_hist hist ptr_e e ver :
+Lemma wp_put_hist cli_γ uid sl_hist hist ptr_e e :
   match last hist with
   | None => True
-  | Some lat => uint.Z lat.(HistEntry.Epoch) < uint.Z e.(HistEntry.Epoch)
+  | Some lat => uint.Z lat.1 < uint.Z e.1
   end →
-  length hist = uint.nat ver →
   {{{
     "Hown_hist" ∷ own_hist cli_γ uid sl_hist hist ∗
-    "Hown_entry" ∷ HistEntry.own ptr_e e ∗
-    "#His_key" ∷ is_my_key cli_γ uid ver e.(HistEntry.Epoch) e.(HistEntry.HistVal)
+    "Hown_entry" ∷ own_HistEntry ptr_e e ∗
+    "#His_key" ∷ is_my_key cli_γ uid (W64 $ length hist) e.1 e.2
   }}}
   SliceAppend ptrT (slice_val sl_hist) #ptr_e
   {{{
     sl_hist', RET (slice_val sl_hist');
     "Hown_hist" ∷ own_hist cli_γ uid sl_hist' (hist ++ [e]) ∗
-    "Hown_entry" ∷ HistEntry.own ptr_e e
+    "Hown_entry" ∷ own_HistEntry ptr_e e
   }}}.
 Proof. Admitted.
 
-Definition msv_final (adtr_γ : gname) (ep uid : w64) (lat : option map_val_ty) : iProp Σ.
-Admitted.
-
-Lemma wp_GetHist cli_γ uid sl_hist hist bound_ep (ep : w64) aud_ep adtr_γ :
-  match last hist with
-  | None => True
-  | Some lat => uint.Z lat.(HistEntry.Epoch) ≤ uint.Z bound_ep
-  end →
-  uint.Z ep ≤ uint.Z bound_ep →
-  uint.Z bound_ep < uint.Z aud_ep →
+Lemma wp_GetHist cli_γ uid sl_hist hist (ep : w64) :
   {{{
-    "Hown_hist" ∷ own_hist cli_γ uid sl_hist hist ∗
-    (* even if don't do SelfMon, can always create this from latest Put. *)
-    "#His_bound" ∷ is_my_bound cli_γ uid (W64 $ length hist) bound_ep ∗
-    "#His_audit" ∷ is_audit cli_γ adtr_γ aud_ep
+    "Hown_hist" ∷ own_hist cli_γ uid sl_hist hist
   }}}
   GetHist (slice_val sl_hist) #ep
   {{{
-    (is_reg : bool) (ep' : w64) sl_pk pk, RET (#is_reg, slice_val sl_pk);
+    (is_reg : bool) sl_pk pk, RET (#is_reg, slice_val sl_pk);
     "Hown_hist" ∷ own_hist cli_γ uid sl_hist hist ∗
     "#Hsl_pk" ∷ own_slice_small sl_pk byteT DfracDiscarded pk ∗
-    "#Hmsv" ∷ msv_final adtr_γ ep uid (if is_reg then Some (ep', pk) else None)
+    "%Heq_lat" ∷
+      ⌜ match get_lat hist ep with
+        | None => is_reg = false
+        | Some lat => is_reg = true ∧ pk = lat.2
+        end ⌝
   }}}.
 Proof. Admitted.
 
